feat: fundamental def

LogRel/STLC/OpenClose.lean
@@ -1,14 +1,8 @@
 
 
+import Mathlib.Data.Set.Insert
 import LogRel.STLC.Basic
-@[simp]
-def opening (i : ℕ) (v : Expr) : Expr → Expr
-  | .bvar j => if j = i then v else .bvar j
-  | .fvar x => .fvar x
-  | .lam e => .lam (opening (i + 1) v e)
-  | .app f arg => .app (opening i v f) (opening i v arg)
-  | .unit => .unit
-
+import LogRel.STLC.Env
 @[simp]
 def closedb_at (e : Expr) (i : ℕ) : Prop :=
   match e with
@@ -19,6 +13,18 @@ def closedb_at (e : Expr) (i : ℕ) : Prop :=
   | .unit => true
 
 @[simp]
+def lc e :=
+  closedb_at e 0
+
+@[simp]
+def opening (i : ℕ) (v : Expr) : Expr → Expr
+  | .bvar j => if j = i then v else .bvar j
+  | .fvar x => .fvar x
+  | .lam e => .lam (opening (i + 1) v e)
+  | .app f arg => .app (opening i v f) (opening i v arg)
+  | .unit => .unit
+
+@[simp]
 def subst (x : ℕ) (v : Expr) : Expr -> Expr
   | .bvar i => .bvar i
   | .fvar y => if x = y then v else .fvar y
@@ -26,6 +32,51 @@ def subst (x : ℕ) (v : Expr) : Expr -> Expr
   | .app f arg => .app (subst x v f) (subst x v arg)
   | .unit => .unit
 
+abbrev Subst :=
+  List Expr
+
 @[simp]
-def lc e :=
-  closedb_at e 0
+def substs (γs : Subst) : Expr -> Expr
+  | .bvar i => .bvar i
+  | .fvar y => (getr y γs).elim (.fvar y) id
+  | .lam e => .lam (substs γs e)
+  | .app f arg => .app (substs γs f) (substs γs arg)
+  | .unit => .unit
+
+@[simp]
+def fv : Expr → Set ℕ
+  | .bvar _ => ∅
+  | .fvar x => { x }
+  | .lam e => fv e
+  | .app f arg => fv f ∪ fv arg
+  | .unit => ∅
+
+theorem subst_intro : ∀ x e v i, x ∉ fv e → subst x v (opening i (.fvar x) e) = opening i v e :=
+  by
+  intros x e _ i HFv
+  induction e generalizing i with
+  | bvar j =>
+    by_cases HEq : j = i
+    . simp [HEq]
+    . simp [if_neg HEq]
+  | fvar y =>
+    simp; intro HEq
+    rw [HEq] at HFv
+    nomatch HFv
+  | lam _ IH => simp; apply IH; apply HFv
+  | app _ _ IH₀ IH₁ =>
+    simp; simp at HFv; constructor
+    apply IH₀; apply HFv.left
+    apply IH₁; apply HFv.right
+  | unit => simp
+
+theorem substs_empty : ∀ e, substs [] e = e := by
+  intro e
+  induction e
+  case bvar => rfl
+  case fvar => rfl
+  case lam IH => simp; apply IH
+  case app IH₀ IH₁ =>
+    simp; constructor
+    apply IH₀; apply IH₁
+  case unit => rfl
