LogRel/STLC/SN.lean
@@ -17,25 +17,28 @@ theorem SN_impl_halts : ∀ e τ, SN e τ → halts e := by
   case unit => apply HSN
   case arrow => apply HSN.left
 
-theorem halts_reduction : ∀ e₀ e₁, step e₀ e₁ → (halts e₀ ↔ halts e₁) :=
+theorem halts_step : ∀ e₀ e₁, step e₀ e₁ → (halts e₀ ↔ halts e₁) :=
   by
   intros e₀ e₁ Hstep
   constructor
-  . admit
-  . admit
+  . admit -- need determinstic
+  . intro Hhalts
+    have ⟨v, Hvalue, Hstepn⟩ := Hhalts
+    exists v; constructor; apply Hvalue
+    apply stepn.multi; apply Hstep; apply Hstepn
 
-theorem SN_reduction : ∀ e₀ e₁ τ, step e₀ e₁ → (SN e₀ τ ↔ SN e₁ τ) :=
+theorem SN_step : ∀ e₀ e₁ τ, step e₀ e₁ → (SN e₀ τ ↔ SN e₁ τ) :=
   by
   intros e₀ e₁ τ Hstep
   constructor
   . intros HSN₀
     induction τ generalizing e₀ e₁
     case unit =>
-      apply (halts_reduction _ _ _).mp
+      apply (halts_step _ _ _).mp
       apply HSN₀; apply Hstep
     case arrow IHa IHb =>
       constructor
-      . apply (halts_reduction _ _ _).mp
+      . apply (halts_step _ _ _).mp
         apply HSN₀.left; apply Hstep
       . intro arg HSN₁
         apply IHb
@@ -44,38 +47,75 @@ theorem SN_reduction : ∀ e₀ e₁ τ, step e₀ e₁ → (SN e₀ τ ↔ SN e
   . intros HSN₀
     induction τ generalizing e₀ e₁
     case unit =>
-      apply (halts_reduction _ _ _).mpr
+      apply (halts_step _ _ _).mpr
       apply HSN₀; apply Hstep
     case arrow IHa IHb =>
       constructor
-      . apply (halts_reduction _ _ _).mpr
+      . apply (halts_step _ _ _).mpr
         apply HSN₀.left; apply Hstep
       . intro arg HSN₁
         apply IHb
         apply step_appl; apply Hstep
         apply HSN₀.right; apply HSN₁
 
-abbrev Subst :=
-  List Expr
+theorem SN_stepn : ∀ e₀ e₁ τ, stepn e₀ e₁ → (SN e₀ τ ↔ SN e₁ τ) :=
+  by
+  intros e₀ e₁ τ Hstepn
+  induction Hstepn
+  case refl => rfl
+  case multi Hstep _ IH => rw [← IH]; apply SN_step; apply Hstep
 
-@[simp]
-def SN_Env : Subst → TEnv → Prop
-  | [], [] => true
-  | v :: vs, τ :: τs => SN v τ ∧ SN_Env vs τs
-  | _, _ => false
+inductive SN_Env : Subst → TEnv → Prop
+  | nil : SN_Env [] []
+  | cons : ∀ γ γs τ τs, SN γ τ → SN_Env γs τs → SN_Env (γ :: γs) (τ :: τs)
 
-@[simp]
-def substs : Subst → Expr → Expr
-  | [], e => e
-  | γ :: γs, e => substs γs (subst γs.length γ e)
+theorem SN_Env_impl_length_eq : ∀ γs τs, SN_Env γs τs → γs.length = τs.length :=
+  by
+  intros γs τs HSNΓ
+  induction HSNΓ
+  case nil => rfl
+  case cons IH => simp; apply IH
 
-theorem typing_impl_SN : ∀ Γ e τ γs, typing Γ e τ → SN_Env γs Γ → SN (substs γs e) τ :=
+theorem fundamental : ∀ Γ e τ γs, typing Γ e τ → SN_Env γs Γ → SN (substs γs e) τ :=
   by
   intros Γ e τ γs Hτ HSNΓ
   induction Hτ generalizing γs
-  case fvar => admit
-  case lam => admit
-  case app => admit
-  case unit => admit
+  case fvar Γ x _ Hbinds =>
+    induction HSNΓ
+    case nil => nomatch Hbinds
+    case cons γ γs τ τs HSN HSNΓ IH =>
+      simp; simp at Hbinds
+      rw [SN_Env_impl_length_eq _ _ HSNΓ]
+      by_cases HEq : (τs.length = x)
+      . simp [if_pos HEq]
+        simp [if_pos HEq] at Hbinds
+        rw [← Hbinds]; apply HSN
+      . simp [if_neg HEq]
+        simp [if_neg HEq] at Hbinds
+        apply IH; apply Hbinds
+  case lam e _ _ _ HFv IH =>
+    constructor; exists substs γs (.lam e)
+    constructor; constructor
+    apply stepn.refl
+    intro arg HSN
+    have ⟨v, Hvalue, Hstepn⟩ := SN_impl_halts _ _ HSN
+    apply (SN_stepn _ _ _ _).mpr; apply IH (v :: γs); apply SN_Env.cons
+    apply (SN_stepn _ _ _ _).mp; apply HSN; apply Hstepn; apply HSNΓ
+    apply stepn_trans; apply stepn_appr; apply Hstepn; constructor
+    apply stepn.multi; apply step.step𝕄 id; apply ctx𝕄.hole; apply head.app; apply Hvalue
+    rw [← SN_Env_impl_length_eq _ _ HSNΓ, ← subst_intro γs.length]
+    all_goals admit
+  case app IH₀ IH₁ =>
+    apply (IH₀ _ HSNΓ).right
+    apply IH₁ _ HSNΓ
+  case unit =>
+    exists .unit
+    constructor
+    . constructor
+    . apply stepn.refl
 
-theorem normalization : ∀ e τ, typing [] e τ → halts e := by admit
+theorem normalization : ∀ e τ, typing [] e τ → halts e :=
+  by
+  intros e τ Hτ
+  apply SN_impl_halts; rw [← substs_empty e]
+  apply fundamental; apply Hτ; apply SN_Env.nil
