LogRel/STLC/SmallStep.lean
@@ -20,13 +20,48 @@ inductive ctx𝕄 : Ctx → Prop where
   | cons𝔹 : ∀ B M, ctx𝔹 B → ctx𝕄 M → ctx𝕄 (B ∘ M)
 
 inductive head : Expr → Expr → Prop where
-  | app₁ : ∀ e v, value v → head (.app (.lam e) v) (opening 0 v e)
+  | app : ∀ e v, value v → head (.app (.lam e) v) (opening 0 v e)
 
 inductive step : Expr → Expr → Prop where
   | step𝕄 : ∀ M e₀ e₁, ctx𝕄 M → head e₀ e₁ → step M⟦e₀⟧ M⟦e₁⟧
 
 inductive stepn : Expr → Expr → Prop
   | refl : ∀ e, stepn e e
-  | trans : ∀ e₁ e₂ e₃, stepn e₁ e₂ → step e₂ e₃ → stepn e₁ e₃
+  | multi : ∀ e₁ e₂ e₃, step e₁ e₂ → stepn e₂ e₃ → stepn e₁ e₃
 
-theorem step_appl : ∀ e₀ e₁ arg, step e₀ e₁ → step (.app e₀ arg) (.app e₁ arg) := by admit
+theorem step_appl : ∀ e₀ e₁ arg, step e₀ e₁ → step (.app e₀ arg) (.app e₁ arg) :=
+  by
+  intros e₀ e₁ arg Hstep
+  cases Hstep
+  case step𝕄 M e₀ e₁ HM Hhead =>
+    apply step.step𝕄 (fun X => .app (M X) arg)
+    apply ctx𝕄.cons𝔹 (fun X => .app X arg)
+    apply ctx𝔹.appl; apply HM; apply Hhead
+
+theorem step_appr : ∀ e₀ e₁ v, step e₀ e₁ → value v → step (.app v e₀) (.app v e₁) :=
+  by
+  intros e₀ e₁ v Hstep Hvalue
+  cases Hstep
+  case step𝕄 M e₀ e₁ HM Hhead =>
+    apply step.step𝕄 (fun X => .app v (M X))
+    apply ctx𝕄.cons𝔹 (fun X => .app v X)
+    apply ctx𝔹.appr; apply Hvalue; apply HM; apply Hhead
+
+theorem stepn_appr : ∀ e₀ e₁ v, stepn e₀ e₁ → value v → stepn (.app v e₀) (.app v e₁) :=
+  by
+  intros e₀ e₁ v Hstep Hvalue
+  induction Hstep
+  case refl => apply stepn.refl
+  case multi Hstep _ IH =>
+    apply stepn.multi
+    apply step_appr; apply Hstep; apply Hvalue
+    apply IH
+
+theorem stepn_trans : ∀ e₁ e₂ e₃, stepn e₁ e₂ → stepn e₂ e₃ → stepn e₁ e₃ :=
+  by
+  intros e₀ e₁ e₃ H₁ H₂
+  induction H₁
+  case refl => apply H₂
+  case multi H₃ _ IH =>
+    apply stepn.multi
+    apply H₃; apply IH; apply H₂
