LogRel/STLC/Env.lean
@@ -1,0 +1,12 @@
+
+
+import Mathlib.Data.Nat.Basic
+@[simp]
+def getr {α : Type} (x : ℕ) (l : List α) : Option α :=
+  match l with
+  | [] => none
+  | head :: tails => if tails.length == x then some head else getr x tails
+
+@[simp]
+def binds {α : Type} (x : ℕ) (a : α) (l : List α) :=
+  getr x l = some a
